examples/conn/proofs/base.v
@@ -55,8 +55,17 @@ Lemma connected_public_key ps skI skR rl cs :
   connected ps skI skR rl cs -∗
   release_token (si_share_of rl cs) -∗
   public (si_key cs) -∗
-  ◇ compromised_session rl cs.
+  ◇ compromised rl cs.
 Proof. exact: GenConn.connected_public_key. Qed.
+
+Lemma connected_public_key_or ps skI skR rl cs P :
+  connected ps skI skR rl cs -∗
+  release_token (si_share_of rl cs) -∗
+  public (si_key cs) ∨ P -∗
+  connected ps skI skR rl cs ∗
+  release_token (si_share_of rl cs) ∗
+  ◇ (compromised rl cs ∨ P).
+Proof. exact: GenConn.connected_public_key_or. Qed.
 
 Lemma connected_released_session ps skI skR rl cs :
   connected ps skI skR rl cs -∗
@@ -74,11 +83,11 @@ Lemma connected_ok ps skI skR rl cs :
   secret skR -∗
   minted skI -∗
   minted skR -∗
-  ◇ □ ¬ compromised_session rl cs.
+  ◇ □ ¬ compromised rl cs.
 Proof. exact: GenConn.connected_ok. Qed.
 
 Lemma session_failed_failure rl si :
-  compromised_session rl si  ⊢ GenConn.failure (si_init si) (si_resp si).
+  compromised rl si  ⊢ GenConn.failure (si_init si) (si_resp si).
 Proof. exact: GenConn.session_failed_failure. Qed.
 
 Lemma connected_failure ps skI skR rl cs :
